Lsc/Lib/Wei/Eval.lean
@@ -23,14 +23,16 @@ def addCheckedNat (a : Wei) (n : Nat) : Except ArithError Wei :=
 abbrev Wei.canAddNat (w : Wei) (n : Nat) : Prop := w.raw.toNat + n < 2 ^ 256
 
 @[simp]
-theorem addCheckedNat_ok (a : Wei) (n : Nat) (h : a.canAddNat n) :
+theorem addCheckedNat_ok (a : Wei) (n : Nat) (h : Wei.canAddNat a n) :
     addCheckedNat a n = .ok ⟨BitVec.ofNat 256 (a.raw.toNat + n)⟩ := by
-  simp [addCheckedNat, UInt256.addCheckedNat, h, Except.map]
+  unfold Wei.canAddNat at h
+  simp [addCheckedNat, UInt256.addCheckedNat_ok a.raw n h, Except.map]
 
 @[simp]
-theorem addCheckedNat_error (a : Wei) (n : Nat) (h : ¬ a.canAddNat n) :
+theorem addCheckedNat_error (a : Wei) (n : Nat) (h : ¬ Wei.canAddNat a n) :
     addCheckedNat a n = .error .Overflow := by
-  simp [addCheckedNat, UInt256.addCheckedNat, h, Except.map]
+  unfold Wei.canAddNat at h
+  simp [addCheckedNat, UInt256.addCheckedNat_error a.raw n h, Except.map]
 
 variable {S E Err : Type} [ContractErrors Err] [dsl : ContractDSL S E Err]
 
